tests/lean/run/aexp.lean
@@ -1,0 +1,70 @@
+namespace imp
+open tactic
+
+@[reducible]
+def uname := string
+
+inductive aexp
+| val   : nat → aexp
+| var   : uname → aexp
+| plus  : aexp → aexp → aexp
+| times : aexp → aexp → aexp
+
+instance : decidable_eq aexp :=
+by mk_dec_eq_instance
+
+@[reducible]
+def value := nat
+
+def state := uname → value
+
+open aexp
+
+def aval : aexp → state → value
+| (val n)      s := n
+| (var x)      s := s x
+| (plus a₁ a₂) s := aval a₁ s + aval a₂ s
+| (times a₁ a₂) s := aval a₁ s * aval a₂ s
+
+example : aval (plus (val 3) (var "x")) (λ x, 0) = 3 :=
+rfl
+
+def updt (s : state) (x : uname) (v : value) : state :=
+λ y, if x = y then v else s y
+
+def asimp_const : aexp → aexp
+| (val n)      := val n
+| (var x)      := var x
+| (plus a₁ a₂) :=
+  match asimp_const a₁, asimp_const a₂ with
+  | val n₁, val n₂ := val (n₁ + n₂)
+  | b₁,     b₂     := plus b₁ b₂
+  end
+| (times a₁ a₂) :=
+  match asimp_const a₁, asimp_const a₂ with
+  | val n₁, val n₂ := val (n₁ * n₂)
+  | b₁,     b₂     := times b₁ b₂
+  end
+
+example : asimp_const (plus (plus (val 2) (val 3)) (var "x")) = plus (val 5) (var "x") :=
+rfl
+
+attribute [ematch] asimp_const aval
+
+-- set_option trace.smt.ematch true
+
+meta def not_done : tactic unit := fail_if_success now
+
+lemma aval_asimp_const (a : aexp) (s : state) : aval (asimp_const a) s = aval a s :=
+begin [smt]
+ induction a,
+ all_goals {destruct (asimp_const a), all_goals {destruct (asimp_const a_1), eblast}}
+end
+
+example (a : aexp) (s : state) : aval (asimp_const a) s = aval a s :=
+begin [smt]
+ induction a,
+ all_goals {destruct (asimp_const a), all_goals {destruct (asimp_const a_1), eblast_using [asimp_const, aval]}}
+end
+
+end imp
